candle/prover/compute/compute_evalProofScript.sml
@@ -541,39 +541,22 @@ Proof
       Cases_on ‘∃n. y = Num n’ \\ fs []
       >- (
         gvs [do_arith_def, st_ex_return_def, cval2term_def]
-        \\ qmatch_asmsub_abbrev_tac ‘_ |- cval2term p === A’
-        \\ qmatch_asmsub_abbrev_tac ‘_ |- cval2term q === B’
-        \\ ‘(thy,[]) |- _CVAL_NUM (_NUMERAL (num2bit (m + n))) ===
-                        _CVAL_ADD A B’
-          suffices_by (
-            rw [Abbr ‘A’, Abbr ‘B’]
-            \\ resolve_then Any irule sym_equation replaceL2
-            \\ first_x_assum (irule_at Any)
-            \\ resolve_then Any irule sym_equation replaceL1
-            \\ first_x_assum (irule_at Any)
-            \\ fs [cval2term_def, sym_equation])
-        \\ unabbrev_all_tac
-        \\ ‘(thy,[]) |- _CVAL_ADD (_CVAL_NUM (num2bit m))
-                                  (_CVAL_NUM (num2bit n)) ===
-                        _CVAL_NUM (num2bit (m + n))’
-          suffices_by (
-            strip_tac
-            \\ irule_at Any replaceL2
-            \\ resolve_then Any (irule_at Any) NUMERAL_eqn sym_equation
-            \\ fs [num2bit_term_ok]
-            \\ resolve_then Any irule trans_equation_simple sym_equation
-            \\ first_x_assum (irule_at Any)
-            \\ irule MK_COMB_simple \\ simp []
-            \\ irule_at Any MK_COMB_simple
-            \\ simp [proves_REFL, compute_thy_ok_terms_ok, sym_equation,
-                     cval2term_def]
-            \\ DEP_REWRITE_TAC [MK_COMB_simple]
-            \\ rw [compute_thy_ok_terms_ok, proves_REFL, NUMERAL_eqn,
-                   sym_equation, num2bit_term_ok])
-        \\ irule replaceR2
-        \\ irule_at Any ADD_num2bit
-        \\ rw [CVAL_ADD_eqn1, sym_equation, compute_thy_ok_def,
-               num2bit_term_ok])
+        \\ ‘(thy,[]) |- cval2term p === _CVAL_NUM (num2bit m)’
+          by (irule trans_equation_simple \\ first_x_assum (irule_at Any)
+              \\ simp [MK_COMB_simple, proves_REFL, compute_thy_ok_terms_ok,
+                       NUMERAL_eqn, num2bit_term_ok])
+        \\ ‘(thy,[]) |- cval2term q === _CVAL_NUM (num2bit n)’
+          by (irule trans_equation_simple \\ first_x_assum (irule_at Any)
+              \\ simp [MK_COMB_simple, proves_REFL, compute_thy_ok_terms_ok,
+                       NUMERAL_eqn, num2bit_term_ok])
+        \\ resolve_then Any irule sym_equation replaceL2
+        \\ first_x_assum (irule_at Any)
+        \\ resolve_then Any irule sym_equation replaceL1
+        \\ first_x_assum (irule_at Any)
+        \\ resolve_then Any irule sym_equation replaceR2
+        \\ irule_at Any NUMERAL_eqn \\ simp [num2bit_term_ok]
+        \\ irule replaceL2 \\ irule_at Any ADD_num2bit
+        \\ rw [CVAL_ADD_eqn1, sym_equation, num2bit_term_ok])
       \\ ‘cval_value y’
         by rw [compute_eval_value, SF SFY_ss]
       \\ ‘∃p1 q1. y = Pair p1 q1’
@@ -587,8 +570,7 @@ Proof
       \\ first_x_assum (irule_at Any)
       \\ resolve_then Any irule sym_equation replaceL1
       \\ first_x_assum (irule_at Any)
-      \\ rw [CVAL_ADD_eqn2, cval2term_term_ok, num2bit_term_ok, NUMERAL_eqn,
-             compute_thy_ok_terms_ok, term_ok_def, Ntimes has_type_cases 2])
+      \\ rw [CVAL_ADD_eqn2, num2bit_term_ok, compute_thy_ok_terms_ok])
     \\ Cases_on ‘∃n. y = Num n’ \\ gs []
     >- (
       gvs [cval2term_def, do_arith_def, st_ex_return_def]
@@ -606,9 +588,7 @@ Proof
       \\ first_x_assum (irule_at Any)
       \\ resolve_then Any irule sym_equation replaceL1
       \\ first_x_assum (irule_at Any)
-      \\ rw [CVAL_ADD_eqn3, cval2term_term_ok, num2bit_term_ok, NUMERAL_eqn,
-             num2bit_term_ok, compute_thy_ok_terms_ok, term_ok_def,
-             Ntimes has_type_cases 2])
+      \\ rw [CVAL_ADD_eqn3, num2bit_term_ok, compute_thy_ok_terms_ok])
     \\ gvs [cval2term_def, do_arith_def, st_ex_return_def]
     \\ ‘cval_value x’
       by rw [compute_eval_value, SF SFY_ss]
@@ -627,46 +607,29 @@ Proof
     \\ first_x_assum (irule_at Any)
     \\ resolve_then Any irule sym_equation replaceL1
     \\ first_x_assum (irule_at Any)
-    \\ fs [] \\ rw [CVAL_ADD_eqn4, cval2term_term_ok, compute_thy_ok_terms_ok])
+    \\ fs [] \\ rw [CVAL_ADD_eqn4, compute_thy_ok_terms_ok])
   >~ [‘_CVAL_SUB _ _’] >- (
     Cases_on ‘∃m. x = Num m’ \\ fs []
     >- (
       Cases_on ‘∃n. y = Num n’ \\ fs []
       >- (
         gvs [do_arith_def, st_ex_return_def, cval2term_def]
-        \\ qmatch_asmsub_abbrev_tac ‘_ |- cval2term p === A’
-        \\ qmatch_asmsub_abbrev_tac ‘_ |- cval2term q === B’
-        \\ ‘(thy,[]) |- _CVAL_NUM (_NUMERAL (num2bit (m - n))) ===
-                        _CVAL_SUB A B’
-          suffices_by (
-            rw [Abbr ‘A’, Abbr ‘B’]
-            \\ resolve_then Any irule sym_equation replaceL2
-            \\ first_x_assum (irule_at Any)
-            \\ resolve_then Any irule sym_equation replaceL1
-            \\ first_x_assum (irule_at Any)
-            \\ fs [cval2term_def, sym_equation])
-        \\ unabbrev_all_tac
-        \\ ‘(thy,[]) |- _CVAL_SUB (_CVAL_NUM (num2bit m))
-                                  (_CVAL_NUM (num2bit n)) ===
-                        _CVAL_NUM (num2bit (m - n))’
-          suffices_by (
-            strip_tac
-            \\ irule_at Any replaceL2
-            \\ resolve_then Any (irule_at Any) NUMERAL_eqn sym_equation
-            \\ fs [num2bit_term_ok]
-            \\ resolve_then Any irule trans_equation_simple sym_equation
-            \\ first_x_assum (irule_at Any)
-            \\ irule MK_COMB_simple \\ simp []
-            \\ irule_at Any MK_COMB_simple
-            \\ simp [proves_REFL, compute_thy_ok_terms_ok, sym_equation,
-                     cval2term_def]
-            \\ DEP_REWRITE_TAC [MK_COMB_simple]
-            \\ rw [compute_thy_ok_terms_ok, proves_REFL, NUMERAL_eqn,
-                   sym_equation, num2bit_term_ok])
-        \\ irule replaceR2
-        \\ irule_at Any SUB_num2bit
-        \\ rw [CVAL_SUB_eqn1, sym_equation, compute_thy_ok_def,
-               num2bit_term_ok])
+        \\ ‘(thy,[]) |- cval2term p === _CVAL_NUM (num2bit m)’
+          by (irule trans_equation_simple \\ first_x_assum (irule_at Any)
+              \\ simp [MK_COMB_simple, proves_REFL, compute_thy_ok_terms_ok,
+                       NUMERAL_eqn, num2bit_term_ok])
+        \\ ‘(thy,[]) |- cval2term q === _CVAL_NUM (num2bit n)’
+          by (irule trans_equation_simple \\ first_x_assum (irule_at Any)
+              \\ simp [MK_COMB_simple, proves_REFL, compute_thy_ok_terms_ok,
+                       NUMERAL_eqn, num2bit_term_ok])
+        \\ resolve_then Any irule sym_equation replaceL2
+        \\ first_x_assum (irule_at Any)
+        \\ resolve_then Any irule sym_equation replaceL1
+        \\ first_x_assum (irule_at Any)
+        \\ resolve_then Any irule sym_equation replaceR2
+        \\ irule_at Any NUMERAL_eqn \\ simp [num2bit_term_ok]
+        \\ irule replaceL2 \\ irule_at Any SUB_num2bit
+        \\ rw [CVAL_SUB_eqn1, sym_equation, num2bit_term_ok])
       \\ ‘cval_value y’
         by rw [compute_eval_value, SF SFY_ss]
       \\ ‘∃p1 q1. y = Pair p1 q1’
@@ -680,8 +643,7 @@ Proof
       \\ first_x_assum (irule_at Any)
       \\ resolve_then Any irule sym_equation replaceL1
       \\ first_x_assum (irule_at Any)
-      \\ rw [CVAL_SUB_eqn2, cval2term_term_ok, num2bit_term_ok, NUMERAL_eqn,
-             compute_thy_ok_terms_ok, term_ok_def, Ntimes has_type_cases 2])
+      \\ rw [CVAL_SUB_eqn2, num2bit_term_ok, compute_thy_ok_terms_ok])
     \\ Cases_on ‘∃n. y = Num n’ \\ gs []
     >- (
       gvs [cval2term_def, do_arith_def, st_ex_return_def]
@@ -690,6 +652,11 @@ Proof
       \\ ‘∃p1 q1. x = Pair p1 q1’
         by (Cases_on ‘x’ \\ fs [])
       \\ gvs [cval2term_def, do_arith_def, st_ex_return_def]
+      \\ simp [Once num2bit_def]
+      \\ ‘(thy,[]) |- cval2term q === _CVAL_NUM (num2bit n)’
+        by (irule trans_equation_simple \\ first_x_assum (irule_at Any)
+            \\ simp [MK_COMB_simple, proves_REFL, compute_thy_ok_terms_ok,
+                     num2bit_term_ok, NUMERAL_eqn])
       \\ ‘term_ok (sigof thy) (cval2term p1) ∧
           term_ok (sigof thy) (cval2term q1)’
         by (qpat_x_assum ‘_ |- _ === _CVAL_PAIR _ _’ assume_tac
@@ -699,9 +666,7 @@ Proof
       \\ first_x_assum (irule_at Any)
       \\ resolve_then Any irule sym_equation replaceL1
       \\ first_x_assum (irule_at Any)
-      \\ rw [CVAL_SUB_eqn3, cval2term_term_ok, num2bit_term_ok, NUMERAL_eqn,
-             num2bit_term_ok, compute_thy_ok_terms_ok, term_ok_def,
-             Ntimes has_type_cases 2])
+      \\ rw [CVAL_SUB_eqn3, num2bit_term_ok, compute_thy_ok_terms_ok])
     \\ gvs [cval2term_def, do_arith_def, st_ex_return_def]
     \\ ‘cval_value x’
       by rw [compute_eval_value, SF SFY_ss]
@@ -720,7 +685,90 @@ Proof
     \\ first_x_assum (irule_at Any)
     \\ resolve_then Any irule sym_equation replaceL1
     \\ first_x_assum (irule_at Any)
-    \\ fs [] \\ rw [CVAL_SUB_eqn4, cval2term_term_ok, compute_thy_ok_terms_ok])
+    \\ fs [] \\ rw [CVAL_SUB_eqn4, compute_thy_ok_terms_ok])
+  >~ [‘_CVAL_MUL _ _’] >- (
+    Cases_on ‘∃m. x = Num m’ \\ fs []
+    >- (
+      Cases_on ‘∃n. y = Num n’ \\ fs []
+      >- (
+        gvs [do_arith_def, st_ex_return_def, cval2term_def]
+        \\ ‘(thy,[]) |- cval2term p === _CVAL_NUM (num2bit m)’
+          by (irule trans_equation_simple \\ first_x_assum (irule_at Any)
+              \\ simp [MK_COMB_simple, proves_REFL, compute_thy_ok_terms_ok,
+                       NUMERAL_eqn, num2bit_term_ok])
+        \\ ‘(thy,[]) |- cval2term q === _CVAL_NUM (num2bit n)’
+          by (irule trans_equation_simple \\ first_x_assum (irule_at Any)
+              \\ simp [MK_COMB_simple, proves_REFL, compute_thy_ok_terms_ok,
+                       NUMERAL_eqn, num2bit_term_ok])
+        \\ resolve_then Any irule sym_equation replaceL2
+        \\ first_x_assum (irule_at Any)
+        \\ resolve_then Any irule sym_equation replaceL1
+        \\ first_x_assum (irule_at Any)
+        \\ resolve_then Any irule sym_equation replaceR2
+        \\ irule_at Any NUMERAL_eqn \\ simp [num2bit_term_ok]
+        \\ irule replaceL2 \\ irule_at Any MUL_num2bit
+        \\ rw [CVAL_MUL_eqn1, sym_equation, num2bit_term_ok])
+      \\ ‘cval_value y’
+        by rw [compute_eval_value, SF SFY_ss]
+      \\ ‘∃p1 q1. y = Pair p1 q1’
+        by (Cases_on ‘y’ \\ fs [])
+      \\ gvs [cval2term_def, do_arith_def, st_ex_return_def]
+      \\ ‘term_ok (sigof thy) (cval2term p1) ∧
+          term_ok (sigof thy) (cval2term q1)’
+        by (drule_then assume_tac proves_term_ok
+            \\ gs [term_ok_def, equation_def])
+      \\ ‘(thy,[]) |- cval2term p === _CVAL_NUM (num2bit m)’
+        by (irule trans_equation_simple \\ first_x_assum (irule_at Any)
+            \\ simp [MK_COMB_simple, proves_REFL, compute_thy_ok_terms_ok,
+                     NUMERAL_eqn, num2bit_term_ok])
+      \\ simp [Once num2bit_def]
+      \\ resolve_then Any irule sym_equation replaceL2
+      \\ first_x_assum (irule_at Any)
+      \\ resolve_then Any irule sym_equation replaceL1
+      \\ first_x_assum (irule_at Any)
+      \\ rw [CVAL_MUL_eqn2, num2bit_term_ok, compute_thy_ok_terms_ok])
+    \\ Cases_on ‘∃n. y = Num n’ \\ gs []
+    >- (
+      gvs [cval2term_def, do_arith_def, st_ex_return_def]
+      \\ ‘cval_value x’
+        by rw [compute_eval_value, SF SFY_ss]
+      \\ ‘∃p1 q1. x = Pair p1 q1’
+        by (Cases_on ‘x’ \\ fs [])
+      \\ gvs [cval2term_def, do_arith_def, st_ex_return_def]
+      \\ ‘term_ok (sigof thy) (cval2term p1) ∧
+          term_ok (sigof thy) (cval2term q1)’
+        by (qpat_x_assum ‘_ |- _ === _CVAL_PAIR _ _’ assume_tac
+            \\ drule_then assume_tac proves_term_ok
+            \\ gs [term_ok_def, equation_def])
+      \\ ‘(thy,[]) |- cval2term q === _CVAL_NUM (num2bit n)’
+        by (irule trans_equation_simple \\ first_x_assum (irule_at Any)
+            \\ simp [MK_COMB_simple, proves_REFL, compute_thy_ok_terms_ok,
+                     NUMERAL_eqn, num2bit_term_ok])
+      \\ simp [Once num2bit_def]
+      \\ resolve_then Any irule sym_equation replaceL2
+      \\ first_x_assum (irule_at Any)
+      \\ resolve_then Any irule sym_equation replaceL1
+      \\ first_x_assum (irule_at Any)
+      \\ rw [CVAL_MUL_eqn3, num2bit_term_ok, compute_thy_ok_terms_ok])
+    \\ gvs [cval2term_def, do_arith_def, st_ex_return_def]
+    \\ ‘cval_value x’
+      by rw [compute_eval_value, SF SFY_ss]
+    \\ ‘∃p1 q1. x = Pair p1 q1’
+      by (Cases_on ‘x’ \\ fs [])
+    \\ ‘cval_value y’
+      by rw [compute_eval_value, SF SFY_ss]
+    \\ ‘∃p2 q2. y = Pair p2 q2’
+      by (Cases_on ‘y’ \\ fs [])
+    \\ gvs [cval2term_def, do_arith_def, st_ex_return_def]
+    \\ simp [Once num2bit_def]
+    \\ ‘EVERY (term_ok (sigof thy) o cval2term) [p1;q1;p2;q2]’
+      by (imp_res_tac proves_term_ok
+          \\ gs [term_ok_def, equation_def])
+    \\ resolve_then Any irule sym_equation replaceL2
+    \\ first_x_assum (irule_at Any)
+    \\ resolve_then Any irule sym_equation replaceL1
+    \\ first_x_assum (irule_at Any)
+    \\ fs [] \\ rw [CVAL_MUL_eqn4, compute_thy_ok_terms_ok])
   >~ [‘_CVAL_LESS _ _’] >- (
     Cases_on ‘∃m. x = Num m’ \\ fs []
     >- (
